Add more definitions

src/Carte/Core/Exec.lean
@@ -1,7 +1,10 @@
+import Carte.Core.Handler
+import Carte.Core.Wpi
 import Iris.ProofMode
 import Iris.BI.Lib.Fixpoint
 import Iris.BI.BigOp.BigSepList
 import ITree.Definition
+import ITree.Exec
 
 namespace Carte.Core
 
@@ -42,6 +45,46 @@ theorem bi_close_respect (P : α → PROP) [Hsym : Symm R] [Htran : Trans R R R]
   · iexact HP
 
 end bi_close
+
+section handler_adequacy
+
+open ITree.Exec
+
+variable {PROP : Type _} [BI PROP] [BIFUpdate PROP]
+
+/-- Logical adequacy interface for executable handlers with thread-pool side effects. -/
+class EHandlerAdequate {E GE : Effect.{u} } {R σ : Type _}
+    (H : IHandler (PROP := PROP) E) (EH : EHandler E GE R σ) where
+  ehandler_inv : σ → List (((ITree GE R → PROP) → PROP)) → PROP
+  ehandler_adequate :
+    ∀ (G : ITree GE R → PROP) (e : E.I) (s : σ)
+      (Ms : List (((ITree GE R → PROP) → PROP)))
+      (C : ITree GE R → σ → Prop) (k : E.O e → ITree GE R),
+      EH.handle e s k C →
+      ⊢ H.ihandle e (fun a => G (k a)) (fun a => iprop(|={⊤,∅}=> G (k a))) -∗
+          ehandler_inv s Ms -∗
+          |={∅}=> ∃ t' s' M' Ms' Msn,
+            ⌜C t' s'⌝ ∗
+            ⌜(M' :: Ms').Perm (Msn ++ Ms)⌝ ∗
+            ([∗list] M ∈ Msn, M G) ∗
+            ehandler_inv s' Ms' ∗
+            bi_close Eq (fun t'' => iprop(∀ P, M' P ={∅}=∗ P t'')) t'
+  ehandler_inv_proper :
+    ∀ {s s' Ms Ms'}, s = s' → Ms = Ms' →
+      ehandler_inv s Ms ⊢ ehandler_inv s' Ms'
+
+/-- Logical adequacy interface for simple executable handlers. -/
+class SEHandlerAdequate {E : Effect.{u} } {σ : Type _}
+    (H : IHandler (PROP := PROP) E) (EH : SEHandler E σ) where
+  sehandler_inv : σ → PROP
+  sehandler_adequate :
+    ∀ (e : E.I) (s : σ) (C : E.O e → σ → Prop) (Φ1 Φ2 : E.O e → PROP),
+      EH.handle e s C →
+      ⊢ H.ihandle e Φ1 Φ2 -∗
+          sehandler_inv s -∗
+          |={∅}=> ∃ a s', ⌜C a s'⌝ ∗ sehandler_inv s' ∗ Φ1 a
+
+end handler_adequacy
 
 /-- [bi_mono0] : linear monotone closure of a predicate transformer. -/
 def bi_mono0 {PROP : Type _} [BI PROP] {α : Type _} (P : (α → PROP) → PROP) : (α → PROP) → PROP :=
@@ -169,33 +212,132 @@ theorem lfp_tp_nil : ⊢ (lfp_tp F [] : PROP) := by
 theorem lfp_tp_ind (Φ : LeibnizO (List ((α → PROP) → PROP)) → PROP)
     [NonExpansive Φ] :
     ⊢ □ (∀ y, lfp_tpF F (λ x => iprop(Φ x ∧ lfp_tp F x.car)) y -∗ Φ y) -∗
-      ∀ Ms, lfp_tp F Ms.car -∗ Φ Ms := by
-  iintro Hwand %Ms Hlfp
-  sorry
-  -- iapply least_fixpoint_ind (lfp_tpF F)
+      (∀ Ms, lfp_tp F Ms.car -∗ Φ Ms) := by
+  iintro #Hwand %Ms Hlfp
+  iapply least_fixpoint_ind (lfp_tpF (PROP := PROP) F)
+  · iintro !> %y Hlfp; iapply Hwand;
+    iapply lfp_tpF_mono F $$ [] Hlfp
+    iintro !> %Ms Hpre; iapply and_congr_r $$ Hpre
+    simp [lfp_tp]
+  · simp [lfp_tp]; iexact Hlfp
+
+-- Helper function for [lfp_*_perm_*]
+theorem perm_pick_erase {β : Type _} {Ms1 Ms2 : List β} {i : Nat} {M : β}
+    (hperm : Ms1.Perm Ms2) (Hi : Ms2[i]? = some M) :
+    ∃ j, Ms1[j]? = some M ∧ (Ms1.eraseIdx j).Perm (Ms2.eraseIdx i) := by
+  induction hperm generalizing i M with
+  | nil => simp at Hi
+  | cons x hperm ih => cases i with
+    | zero => simp at Hi; subst M; refine ⟨0, ?_, ?_⟩; simp; simpa
+    | succ i =>
+      simp at Hi; rcases ih Hi with ⟨j, Hj, Hperm⟩
+      refine ⟨j + 1, ?_, ?_⟩
+      · simpa [Nat.add_comm, Nat.add_left_comm, Nat.add_assoc] using Hj
+      · simpa [List.eraseIdx_cons_succ] using List.Perm.cons x Hperm
+  | swap x y l => cases i with
+    | zero => simp at Hi; subst M; refine ⟨1, ?_, ?_⟩; simp; simp
+    | succ i => cases i with
+      | zero => simp at Hi; subst M; refine ⟨0, ?_, ?_⟩; simp; simp
+      | succ i =>
+        simp at Hi; refine ⟨i + 2, ?_, ?_⟩
+        · simpa [Nat.add_assoc, Nat.add_comm, Nat.add_left_comm] using Hi
+        · simpa [List.eraseIdx, Nat.add_assoc, Nat.add_comm, Nat.add_left_comm]
+            using List.Perm.swap x y (l.eraseIdx i)
+  | trans h₁ h₂ ih₁ ih₂ =>
+      rcases ih₂ Hi with ⟨j₂, Hj₂, Hperm₂⟩
+      rcases ih₁ Hj₂ with ⟨j₁, Hj₁, Hperm₁⟩
+      exact ⟨j₁, Hj₁, List.Perm.trans Hperm₁ Hperm₂⟩
 
 theorem lfp_tpF_perm (Ms1 Ms2 : List ((α → PROP) → PROP))
     (wp1 wp2 : LeibnizO (List ((α → PROP) → PROP)) → PROP)
     (h : Ms1.Perm Ms2) :
-    ⊢ lfp_tpF F wp1 ⟨Ms1⟩ -∗
-      (∀ (Ns1 Ns2 : LeibnizO (List ((α → PROP) → PROP))),
-        ⌜Ns1.car.Perm Ns2.car⌝ -∗ wp1 Ns1 -∗ wp2 Ns2) -∗
-      lfp_tpF F wp2 ⟨Ms2⟩ := by
-  sorry
+    lfp_tpF F wp1 ⟨Ms1⟩ ⊢
+    (∀ (Ns1 Ns2 : LeibnizO (List ((α → PROP) → PROP))),
+      ⌜Ns1.car.Perm Ns2.car⌝ -∗ wp1 Ns1 -∗ wp2 Ns2) -∗
+    lfp_tpF F wp2 ⟨Ms2⟩ := by
+  iintro Htp Hwp; unfold lfp_tpF; iintro %i %M %Hi
+  rcases perm_pick_erase h Hi with ⟨j, Hj, Herase⟩
+  ispecialize Htp $$ %j %M %Hj
+  iapply bi_mono0_mono $$ Htp
+  iintro %x Hstep; icases Hstep with ⟨%G, HFx, Hcont⟩
+  iexists G; isplitl [HFx]; iexact HFx
+  iintro %Ms' HM'; iapply Hwp $$ %⟨Ms' ++ Ms1.eraseIdx j⟩ %⟨Ms' ++ Ms2.eraseIdx i⟩
+  · ipure_intro; simp; exact (List.perm_append_left_iff Ms').2 Herase
+  · iapply Hcont $$ HM'
 
 theorem lfp_tpF_perm_close (Ms1 Ms2 : List ((α → PROP) → PROP))
     (wp : LeibnizO (List ((α → PROP) → PROP)) → PROP)
     (h : Ms1.Perm Ms2) :
-    ⊢ lfp_tpF F wp ⟨Ms1⟩ -∗
-      lfp_tpF F (bi_close (fun a b => a.car.Perm b.car) wp) ⟨Ms2⟩ := by
-  sorry
+    lfp_tpF F wp ⟨Ms1⟩ ⊢
+    lfp_tpF F (bi_close (λ a b => a.car.Perm b.car) wp) ⟨Ms2⟩ := by
+  iintro Htp; iapply lfp_tpF_perm $$ Htp
+  · exact h
+  · iintro %Ns1 %Ns2 %Hperm Hwp; simp only [bi_close]
+    iexists Ns1; isplitr
+    · ipure_intro; exact Hperm.symm
+    · iexact Hwp
 
 theorem lfp_tp_perm (Ms1 Ms2 : List ((α → PROP) → PROP)) (h : Ms1.Perm Ms2) :
     ⊢ lfp_tp F Ms1 -∗ lfp_tp F Ms2 := by
-  sorry
+  letI : NonExpansive λ (Ms : LeibnizO (List ((α → PROP) → PROP))) =>
+    iprop(∀ Ms2, ⌜Ms.car.Perm Ms2⌝ -∗ lfp_tp F Ms2) := ⟨
+      λ n lst1 lst2 Hlst => by
+        refine forall_ne (λ lst => ?_)
+        cases Hlst; rfl
+    ⟩
+  iintro Htp; irevert %Ms2 %h
+  iapply lfp_tp_ind F λ Ms => iprop(∀ Ms2, ⌜Ms.car.Perm Ms2⌝ -∗ lfp_tp F Ms2) $$ [] Htp
+  iintro !> %Ms1 Htp %Ms2 %Hperm; iapply lfp_tp_unfold
+  iapply lfp_tpF_perm F Ms1.car _ _ _ Hperm $$ Htp
+  iintro %Ns1 %Ns2 %Hperm Hw; icases Hw with ⟨H, -⟩
+  iapply H; ipure_intro; exact Hperm
 
 theorem lfp_tp_app (Ms1 Ms2 : List ((α → PROP) → PROP)) :
     ⊢ lfp_tp F Ms1 -∗ lfp_tp F Ms2 -∗ lfp_tp F (Ms1 ++ Ms2) := by
+  letI : NonExpansive λ (Ms : LeibnizO (List ((α → PROP) → PROP))) =>
+    iprop(∀ Ms2, lfp_tp F Ms2 -∗ lfp_tp F (Ms.car ++ Ms2)) := by
+      sorry
+  have Hwrap :
+      ⊢ BI.forall (fun Ms1 : LeibnizO (List ((α → PROP) → PROP)) =>
+            iprop(lfp_tp F Ms1.car -∗ BI.forall (fun Ms2 =>
+              iprop(lfp_tp F Ms2 -∗ lfp_tp F (Ms1.car ++ Ms2))))) -∗
+          BI.forall (fun Ms1 : List ((α → PROP) → PROP) =>
+            iprop(lfp_tp F Ms1 -∗ BI.forall (fun Ms2 =>
+              iprop(lfp_tp F Ms2 -∗ lfp_tp F (Ms1 ++ Ms2))))) := by
+    iintro H %Ms1 Hx1 %Ms2 Hx2
+    iapply H $$ %⟨Ms1⟩ Hx1 %Ms2 Hx2
+  have Hwrap2 :
+      ⊢ BI.forall (fun Ms2 : LeibnizO (List ((α → PROP) → PROP)) =>
+            iprop(lfp_tp F Ms2.car -∗ BI.forall (fun Ms1 =>
+              iprop(lfp_tpF F (fun x =>
+                iprop((∀ Ms, lfp_tp F Ms -∗ lfp_tp F (x.car ++ Ms)) ∧ lfp_tp F x.car)) Ms1 -∗
+                  lfp_tp F (Ms1.car ++ Ms2.car))))) -∗
+          BI.forall (fun Ms2 : List ((α → PROP) → PROP) =>
+            iprop(lfp_tp F Ms2 -∗ BI.forall (fun Ms1 =>
+              iprop(lfp_tpF F (fun x =>
+                iprop((∀ Ms, lfp_tp F Ms -∗ lfp_tp F (x.car ++ Ms)) ∧ lfp_tp F x.car)) Ms1 -∗
+                  lfp_tp F (Ms1.car ++ Ms2))))) := by
+    iintro H %Ms2 Hx2 %Ms1 Hx1
+    iapply H $$ %⟨Ms2⟩ Hx2 %Ms1 Hx1
+  iintro Hx1 Hx2; irevert %Ms1 Hx1 %Ms2 Hx2
+  iapply Hwrap
+  iapply lfp_tp_ind F λ Ms => iprop(∀ Ms2, lfp_tp F Ms2 -∗ lfp_tp F (Ms.car ++ Ms2))
+  iintro !> %Ms1 Hx1 %Ms2 Hx2; irevert %Ms1 Hx1; irevert %Ms2 Hx2
+  letI : NonExpansive λ (Ms : LeibnizO (List ((α → PROP) → PROP))) =>
+      iprop(∀ Ms1, lfp_tpF F (λ x =>
+        iprop((∀ Ms, lfp_tp F Ms -∗ lfp_tp F (x.car ++ Ms)) ∧ lfp_tp F x.car)) Ms1 -∗
+          lfp_tp F (Ms1.car ++ Ms.car)) := ⟨
+        λ n lst1 lst2 Hlst => by
+          refine forall_ne (λ Ms1 => ?_)
+          cases Hlst
+          rfl
+      ⟩
+  iapply Hwrap2
+  iapply lfp_tp_ind F λ Ms => iprop(∀ Ms1, lfp_tpF F (λ x =>
+    iprop((∀ Ms, lfp_tp F Ms -∗ lfp_tp F (x.car ++ Ms)) ∧ lfp_tp F x.car)) Ms1 -∗
+      lfp_tp F (Ms1.car ++ Ms.car))
+  iintro !> %Ms2 Hx2 %Ms1 Hx1; iapply lfp_tp_unfold; unfold lfp_tpF at ⊢; simp
+  iintro %i %M %Hi
   sorry
 
 theorem lfp_tp_cons (M : (α → PROP) → PROP) (Ms : List ((α → PROP) → PROP)) :
@@ -208,10 +350,174 @@ theorem lfp_tp_singleton_mod_elim (M : (α → PROP) → PROP) :
 
 end lfp_tp_lemmas
 
-theorem lfp_tp_intro_of {PROP : Type _} [BI PROP] {α : Type _} [OFE α]
-    (G : (α → PROP) → (α → PROP)) [BIMonoPred G] (x : α) :
+theorem lfp_tp_intro_of {PROP : Type _} [BI PROP] [BIAffine PROP]
+    {α : Type _} [OFE α] [OFE.Discrete α] [OFE.Leibniz α]
+    (G : (α → PROP) → (α → PROP)) [HG : BIMonoPred G] (x : α) :
     ⊢ bi_least_fixpoint G x -∗ lfp_tp G [λ P => P x] := by
+  letI : NonExpansive (fun (x : α) => lfp_tp G [λ P => P x] : α → PROP) := ⟨
+    fun {n x1 x2} Hx => by
+      have Heq : x1 = x2 := OFE.eq_of_eqv (OFE.Discrete.discrete Hx)
+      subst Heq; rfl
+  ⟩
+  irevert %x; iapply least_fixpoint_iter
+  · iintro !> %x HF
+    iapply (lfp_tp_unfold G [λ P => P x]).mpr
+    simp only [lfp_tpF]
+    iintro %i %M %Hi
+    cases i with
+    | zero =>
+      simp at Hi; subst Hi
+      simp only [bi_mono0]
+      iexists (G (fun y => lfp_tp G [λ P => P y]))
+      isplitl [HF]
+      · iexact HF
+      · iintro %y HGy
+        iexists (fun y => lfp_tp G [λ P => P y])
+        isplitl [HGy]
+        · iexact HGy
+        · iintro %Ms' HMs'
+          simp only [List.eraseIdx, List.append_nil]
+          sorry
+    | succ n => simp at Hi
+
+/-! ## Constant-Φ weakest precondition -/
+
+/-- The constant-Φ weakest precondition functional.
+    Unlike `wpiF`, the postcondition Φ is fixed rather than varying. -/
+def wpi_constF {E : Effect} {R : Type _} {PROP : Type _} [BI PROP] [BIFUpdate PROP]
+    (H : IHandler (PROP := PROP) E) (Φ : R → PROP)
+    (wpi : LeibnizO (ITree E R) → PROP) :
+    LeibnizO (ITree E R) → PROP :=
+  λ t => iprop(
+    |={∅}=> match t.car.unfold with
+    | ITreeF.ret r => Φ r
+    | ITreeF.tau t' => wpi ⟨t'⟩
+    | ITreeF.vis i k => H.ihandle i
+        (λ a => wpi ⟨k a⟩)
+        (λ a => iprop(|={⊤,∅}=> wpi ⟨k a⟩))
+  )
+
+section wp_itree_const
+
+variable {E : Effect} {R : Type _} {PROP : Type _} [BI PROP] [BIFUpdate PROP]
+
+instance wpi_constF_ne (H : IHandler (PROP := PROP) E) (Φ : R → PROP) :
+    NonExpansive (wpi_constF H Φ) where
+  ne {_ wp1 wp2} Hwp := by
+    intro t
+    cases h : t.car.unfold <;> simp [wpi_constF, h]
+    case tau t' => exact BIFUpdate.ne.ne <| Hwp ⟨t'⟩
+    case vis i k =>
+      apply BIFUpdate.ne.ne
+      apply OFE.NonExpansive₂.ne (f := H.ihandle i)
+      · intro a; apply Hwp ⟨k a⟩
+      · intro a; apply BIFUpdate.ne.ne <| Hwp ⟨k a⟩
+
+theorem wpi_constF_mono (H : IHandler (PROP := PROP) E) (Φ : R → PROP)
+    (wp1 wp2 : LeibnizO (ITree E R) → PROP) :
+    ⊢ □ (∀ t, wp1 t -∗ wp2 t) -∗
+      ∀ t, wpi_constF H Φ wp1 t -∗ wpi_constF H Φ wp2 t := by
+  iintro #Hwand %t Hwp; unfold wpi_constF
+  cases t.car.unfold <;> simp
+  case ret => iexact Hwp
+  case tau t' => imod Hwp; imodintro; iapply Hwand $$ Hwp
+  case vis i k =>
+    imod Hwp; imodintro; iapply H.ihandle_mono
+    · iintro %a Hk; iapply Hwand $$ Hk
+    · iintro !> %a Hk; imod Hk; imodintro; iapply Hwand $$ Hk
+    · iexact Hwp
+
+instance wp_itree_const_mono (H : IHandler (PROP := PROP) E) (Φ : R → PROP) :
+    BIMonoPred (wpi_constF H Φ) where
+  mono_pred := by
+    iintro %wp1 %wp2 %Hne1 %Hne2 #Hwand %t Hwp
+    iapply wpi_constF_mono H Φ wp1 wp2 $$ [] Hwp
+    iexact Hwand
+  mono_pred_ne.ne n t1 t2 Hdist := by
+    cases Hdist; rfl
+
+/-- The constant-Φ weakest precondition, as the least fixpoint of `wpi_constF`. -/
+def wpi_const (H : IHandler (PROP := PROP) E) (Φ : R → PROP) : ITree E R → PROP :=
+  λ t => bi_least_fixpoint (wpi_constF H Φ) ⟨t⟩
+
+theorem wpi_const_iter (H : IHandler (PROP := PROP) E) (Φ : R → PROP)
+    (P : LeibnizO (ITree E R) → PROP) [NonExpansive P] :
+    ⊢ □ (∀ y, wpi_constF H Φ P y -∗ P y) -∗
+      ∀ t, bi_least_fixpoint (wpi_constF H Φ) t -∗ P t :=
+  @least_fixpoint_iter _ _ _ _ (wpi_constF H Φ) P _
+
+end wp_itree_const
+
+/-! ## Thread-pool weakest precondition -/
+
+/-- The thread-pool weakest precondition, built from `wpi_constF` and `lfp_tp`. -/
+def wpi_tp {E : Effect} {R : Type _} {PROP : Type _} [BI PROP] [BIFUpdate PROP]
+    (H : IHandler (PROP := PROP) E)
+    (Ms : List (((LeibnizO (ITree E R) → PROP) → PROP)))
+    (Φ : R → PROP) : PROP :=
+  lfp_tp (wpi_constF H Φ) Ms
+
+section wpi_tp_section
+
+variable {E : Effect} {R : Type _} {PROP : Type _} [BI PROP] [BIFUpdate PROP] [BIAffine PROP]
+
+theorem wpi_tp_intro (t : ITree E R) (H : IHandler (PROP := PROP) E) (Φ : R → PROP) :
+    (WPi t @> H {{ Φ }}) ⊢ wpi_tp H [λ P => P ⟨t⟩] Φ := by
   sorry
 
+theorem wpi_tp_perm (H : IHandler (PROP := PROP) E) (Φ : R → PROP)
+    (Ms1 Ms2 : List (((LeibnizO (ITree E R) → PROP) → PROP)))
+    (h : Ms1.Perm Ms2) :
+    wpi_tp H Ms1 Φ ⊣⊢ wpi_tp H Ms2 Φ := by
+  simp only [wpi_tp]
+  isplit <;> iintro Htp
+  · iapply lfp_tp_perm (wpi_constF H Φ) Ms1 Ms2 h $$ Htp
+  · iapply lfp_tp_perm (wpi_constF H Φ) Ms2 Ms1 h.symm $$ Htp
+
+end wpi_tp_section
+
+/-! ## Adequacy -/
+
+section wpi_adequate
+
+open ITree.Exec
+
+variable {E : Effect.{u} } {R : Type u} {σ : Type _}
+  {PROP : Type _} [BI PROP] [BIFUpdate PROP] [BIAffine PROP]
+
+theorem wpi_adequate_ind (Φ : R → PROP) (H : IHandler (PROP := PROP) E)
+    (EH : EHandler E E R σ) [A : EHandlerAdequate (PROP := PROP) H EH]
+    (t : ITree E R) (s : σ)
+    (Ms : List (((LeibnizO (ITree E R) → PROP) → PROP)))
+    (Mss : List (((ITree E R → PROP) → PROP)))
+    (M : (LeibnizO (ITree E R) → PROP) → PROP)
+    (C : ITree E R → σ → Prop)
+    (Hexec : exec EH t s C)
+    (HMs : Ms.Perm (M :: Mss.map (λ M' P => M' (λ t => P ⟨t⟩)))) :
+    ⊢ wpi_tp H Ms Φ -∗
+      A.ehandler_inv s Mss -∗
+      (∀ P, M P ={∅}=∗ P ⟨t⟩) -∗
+      |={∅}=> ∃ t' s' Ms' M',
+        ⌜C t' s'⌝ ∗
+        A.ehandler_inv s' Ms' ∗
+        bi_close Eq (λ t'' => iprop(∀ P, M' P ={∅}=∗ P t'')) ⟨t'⟩ ∗
+        wpi_tp H (M' :: Ms'.map (λ M'' P => M'' (λ t => P ⟨t⟩))) Φ := by
+  sorry
+
+theorem wpi_adequate (Φ : R → PROP) (H : IHandler (PROP := PROP) E)
+    (EH : EHandler E E R σ) [A : EHandlerAdequate (PROP := PROP) H EH]
+    (t : ITree E R) (s : σ)
+    (C : ITree E R → σ → Prop) (m : CoPset)
+    (Hexec : exec EH t s C) :
+    ⊢ iprop(|={m,∅}=> wpi H t (λ v => iprop(|={∅,m}=> Φ v))) -∗
+      A.ehandler_inv s [] -∗
+      |={m, ∅}=> ∃ t' s' Ms' M',
+      ⌜C t' s'⌝ ∗
+      A.ehandler_inv s' Ms' ∗
+      bi_close Eq (λ t'' => iprop(∀ P, M' P ={∅}=∗ P t'')) ⟨t'⟩ ∗
+      wpi_tp H (M' :: Ms'.map (λ M'' P => M'' (λ t => P ⟨t⟩))) (λ v => iprop(|={∅,m}=> Φ v)) := by
+  sorry
+
+end wpi_adequate
 
 end Carte.Core
